More work sketching out the type inference proof

type_checker/inferSoundScript.sml
@@ -3,26 +3,14 @@ open MiniMLTheory MiniMLTerminationTheory inferTheory unifyTheory;
 
 val _ = new_theory "inferSound";
 
-val convert_t_def = Define `
-(convert_t (Infer_Tvar_db n) = Tvar_db n) ∧
-(convert_t (Infer_Tapp ts tc) = Tapp (convert_ts ts) tc) ∧
-(convert_ts [] = []) ∧
-(convert_ts (t::ts) = convert_t t :: convert_ts ts)`;
+val flookup_thm = Q.prove (
+`!f x v. ((FLOOKUP f x = NONE) = x ∉ FDOM f) ∧
+         ((FLOOKUP f x = SOME v) = x ∈ FDOM f ∧ (f ' x = v))`,
+rw [FLOOKUP_DEF]);
 
-val convert_env_def = Define `
-(convert_env s [] = []) ∧
-(convert_env s ((n,(tvs,t))::env) =
-  (n,(tvs,convert_t (apply_subst_t s t)))::convert_env s env)`;
-
-val convert_menv_def = Define `
-(convert_menv s [] = []) ∧
-(convert_menv s ((mn,env)::menv) =
-  ((mn, convert_env s env)::convert_menv s menv))`;
-
-val convert_tenv_def = Define `
-(convert_tenv s [] = Empty) ∧
-(convert_tenv s ((n,(tvs,t))::tenv) = 
-  Bind_name n tvs (convert_t (apply_subst_t s t)) (convert_tenv s tenv))`;
+val count_add1 = Q.prove (
+`!n. count (n + 1) = n INSERT count n`,
+metis_tac [COUNT_SUC, arithmeticTheory.ADD1]);
 
 val st_ex_bind_success = Q.prove (
 `!f g st st' v. 
@@ -34,46 +22,181 @@ rw [] >>
 cases_on `q` >>
 rw []);
 
-(*
-val infer_invariant_def = Define `
-infer_invariant st = T`;
+val fresh_uvar_success = Q.prove (
+`!st t st'. 
+  (fresh_uvar st = (Success t, st')) =
+  ((t = Infer_Tuvar st.next_uvar) ∧
+   (st' = st with next_uvar := st.next_uvar + 1))`,
+rw [fresh_uvar_def] >>
+metis_tac []);
 
+val apply_subst_success = Q.prove (
+`!t1 st1 t2 st2.
+  (apply_subst t1 st1 = (Success t2, st2))
+  =
+  ((st2 = st1 with subst := t_collapse st1.subst) ∧
+   (t2 = apply_subst_t (t_collapse st1.subst) t1))`,
+rw [LET_THM, apply_subst_def] >>
+eq_tac >>
+rw []);
+
+val check_t_def = tDefine "check_t" `
+(check_t n uvars (Infer_Tuvar v) = v ∈ uvars) ∧
+(check_t n uvars (Infer_Tvar_db n') = 
+  n' < n) ∧
+(check_t n uvars (Infer_Tapp ts tc) = EVERY (check_t n uvars) ts)`
+(WF_REL_TAC `measure (infer_t_size o SND o SND)` >>
+ rw [] >>
+ induct_on `ts` >>
+ rw [infer_t_size_def] >>
+ res_tac >>
+ decide_tac);
+
+val check_menv_def = Define `
+check_menv menv =
+  EVERY (\(mn,env). EVERY (\(x, (tvs,t)). check_t tvs {} t) env) menv`;
+
+val convert_t_def = tDefine "convert_t" `
+(convert_t (Infer_Tvar_db n) = Tvar_db n) ∧
+(convert_t (Infer_Tapp ts tc) = Tapp (MAP convert_t ts) tc)`
+(WF_REL_TAC `measure infer_t_size` >>
+ rw [] >>
+ induct_on `ts` >>
+ rw [infer_t_size_def] >>
+ res_tac >>
+ decide_tac);
+
+val convert_menv_def = Define `
+convert_menv menv = 
+  MAP (\(mn,env). (mn, MAP (\(x,(tvs,t)). (x,(tvs,convert_t t))) env)) menv`;
+
+val (tenv_rel_rules, tenv_rel_ind, tenv_rel_cases) = Hol_reln `
+(!sub. 
+  tenv_rel sub [] Empty) ∧
+(!sub x tvs t env tenv.
+  tenv_rel sub env tenv
+  ⇒
+  tenv_rel sub ((x,(tvs,t))::env) 
+               (Bind_name x tvs (convert_t (apply_subst_t sub t)) tenv)) ∧
+(!sub tvs env tenv.
+  tenv_rel sub env tenv 
+  ⇒
+  tenv_rel sub env (Bind_tvar tvs tenv))`;
+
+val infer_invariant_def = Define `
+infer_invariant st = 
+  (* Only substitute for existing uvars *)
+  (FDOM st.subst ⊆ count st.next_uvar) ∧
+  (* Only uvars that exist can occur in the types substituted in *)
+  (!t. t ∈ FRANGE st.subst ⇒ check_t 0 (count st.next_uvar) t)`;
+
+val sub_ext_def = Define `
+sub_ext dom num_tvs sub ext =
+  (FDOM ext = dom DIFF FDOM sub) ∧
+  (!t. t ∈ FRANGE ext ⇒ check_t num_tvs {} t)`;
+
+val check_convert_freevars = Q.prove (
+`(!tvs uvs t. check_t tvs uvs t ⇒ (uvs = {}) ⇒ check_freevars tvs [] (convert_t t))`,
+ho_match_mp_tac (fetch "-" "check_t_ind") >>
+rw [check_freevars_def, check_t_def, convert_t_def] >>
+fs [EVERY_MEM, MEM_MAP] >>
+metis_tac []);
+
+(*
 val infer_e_sound = Q.prove (
-`(!menv cenv env e st st' sub t.
+`(!menv cenv env e st st' ext tenv t.
     (infer_e menv cenv env e st = (Success t, st')) ∧
+    check_menv menv ∧
     infer_invariant st ∧
-    (sub = t_collapse st'.subst)
+    sub_ext (count st'.next_uvar) (num_tvs tenv) st'.subst ext ∧
+    tenv_rel (st'.subst ⊌ ext) env tenv
     ⇒
-    type_e (convert_menv sub menv) cenv (convert_tenv sub env) e 
-           (convert_t (apply_subst_t sub t))) ∧
- (!menv cenv env es st st' sub ts.
+    type_e (convert_menv menv) cenv tenv e 
+           (convert_t (apply_subst_t (st'.subst ⊌ ext) t))) ∧
+ (!menv cenv env es st st' ext tenv ts.
     (infer_es menv cenv env es st = (Success ts, st')) ∧
+    check_menv menv ∧
     infer_invariant st ∧
-    (sub = t_collapse st'.subst)
+    sub_ext (count st'.next_uvar) (num_tvs tenv) st'.subst ext ∧
+    tenv_rel (st'.subst ⊌ ext) env tenv
     ⇒
-    type_es (convert_menv sub menv) cenv (convert_tenv sub env) es 
-            (MAP (convert_t o apply_subst_t sub) ts)) ∧
- (!menv cenv env pes t1 t2 st st' sub.
+    type_es (convert_menv menv) cenv tenv es 
+            (MAP (convert_t o apply_subst_t (st'.subst ⊌ ext)) ts)) ∧
+ (!menv cenv env pes t1 t2 st st' tenv ext.
     (infer_pes menv cenv env pes t1 t2 st = (Success (), st')) ∧
+    check_menv menv ∧
     infer_invariant st ∧
-    (sub = t_collapse st'.subst)
+    sub_ext (count st'.next_uvar) (num_tvs tenv) st'.subst ext ∧
+    tenv_rel (st'.subst ⊌ ext) env tenv
     ⇒
     T) ∧
- (!menv cenv env funs st st' sub env'.
+ (!menv cenv env funs st st' ext tenv.
     (infer_funs menv cenv env funs st = (Success (), st')) ∧
+    check_menv menv ∧
     infer_invariant st ∧
-    (sub = t_collapse st'.subst)
+    sub_ext (count st'.next_uvar) (num_tvs tenv) st'.subst ext ∧
+    tenv_rel (st'.subst ⊌ ext) env tenv
     ⇒
-    ?env'. type_funs (convert_menv sub menv) cenv (convert_tenv sub env) funs env')`,
+    ?env'. type_funs (convert_menv menv) cenv tenv funs env')`,
 
 ho_match_mp_tac infer_e_ind >>
-rw [infer_e_def, st_ex_return_def, st_ex_bind_success] >>
+rw [infer_e_def, st_ex_return_def, st_ex_bind_success, failwith_def] >>
 ONCE_REWRITE_TAC [type_e_cases] >>
 rw [apply_subst_t_eqn, convert_t_def, Tbool_def, Tint_def, Tunit_def] >|
 
-[fs [fresh_uvar_def] >>
+[fs [fresh_uvar_success] >>
      rw [apply_subst_t_eqn, convert_t_def] >>
+     fs [infer_invariant_def, sub_ext_def, LET_THM, FLOOKUP_FUNION] >>
      every_case_tac >>
-     rw [convert_t_def]
+     rw [convert_t_def] >>
+     fs [flookup_thm, count_add1, FRANGE_DEF, SUBSET_DEF] >>
+     metis_tac [IN_INSERT, check_convert_freevars, prim_recTheory.LESS_REFL],
+
+(* Fn case *)
+rw [Tfn_def]
+ 
+(* Poly LET case (r 15;) *)
+`?tvs t_gen. generalise n 0 t1' = (tvs,t_gen)` 
+        by (cases_on `generalise n 0 t1'` >>
+            rw []) >>
+DISJ1_TAC >>
+fs [apply_subst_thm, get_next_uvar_def] >>
+rw [] >>
+fs [st_ex_bind_success] >>
+rw [] >>
+qexists_tac `convert_t (apply_subst_t sub t1)` >>
+qexists_tac `tvs` >>
+rw [] >|
+[qpat_assum `∀st''''' st'''''' sub' tenv' t'.
+        (infer_e menv cenv env e st''''' = (Success t',st'''''')) ∧
+        tenv_rel sub' env tenv' ∧ infer_invariant st'''''' sub' ⇒
+        type_e (convert_menv menv) cenv tenv' e
+          (convert_t (apply_subst_t sub' t'))`
+            match_mp_tac >>
+     qexists_tac `st` >>
+     qexists_tac `st'''` >>
+     rw [] >|
+     [all_tac,
+      fs [get_next_uvar_def] >>
+          rw [] >>
+          fs [st_ex_bind_success] >>
+          imp_res_tac apply_subst_st >>
+          rw []
+
+ qpat_assum `∀num_gen t1'' st''''' st'''''' sub' tenv' t'.
+        (infer_e menv cenv (bind x (num_gen,t1'') env) e' st''''' =
+         (Success t',st'''''')) ∧
+        tenv_rel sub' (bind x (num_gen,t1'') env) tenv' ∧
+        infer_invariant st'''''' sub' ⇒
+        type_e (convert_menv menv) cenv tenv' e'
+          (convert_t (apply_subst_t sub' t'))` match_mp_tac >>
+     qexists_tac `tvs` >>
+     qexists_tac `t_gen` >>
+     qexists_tac `st''''` >>
+     qexists_tac `st'` >>
+     rw [] >>
+     fs [st_ex_bind_success] >>
+     rw [Once tenv_rel_cases, bind_def, bind_tenv_def]
      *)
+
 val _ = export_theory ();
